coq/LLVMGen/tmp_aux_Vellvm.v
@@ -511,3 +511,208 @@ Section TLE_To_Modul.
 End TLE_To_Modul.
 
 Infix "@" := (modul_app) (at level 60).
+
+(** Facts about [alist] proved in our compiler example for itrees. Should still go to ExtLib **)
+
+From ExtLib Require Import
+     Core.RelDec
+     Data.Map.FMapAList.
+Section alistFacts.
+
+
+  (* Generic facts about alists. To eventually move to ExtLib. *)
+
+  Arguments alist_find {_ _ _ _}.
+
+  Definition alist_In {K R RD V} k m v := @alist_find K R RD V k m = Some v.
+
+  Arguments alist_add {_ _ _ _}.
+  Arguments alist_find {_ _ _ _}.
+  Arguments alist_remove {_ _ _ _}. 
+
+  Context {K V: Type}.
+  Context {RR : @RelDec K (@eq K)}.
+  Context {RRC : @RelDec_Correct K (@eq K) RR}.
+  
+  Lemma In_add_eq:
+    forall k v (m: alist K V),
+      alist_In k (alist_add k v m) v.
+  Proof.
+    intros; unfold alist_add, alist_In; simpl; flatten_goal; [reflexivity | rewrite <- neg_rel_dec_correct in Heq; tauto]. 
+  Qed.
+
+  (* A removed key is not contained in the resulting map *)
+  Lemma not_In_remove:
+    forall (m : alist K V) (k : K) (v: V),
+      ~ alist_In k (alist_remove k m) v.
+  Proof.
+    induction m as [| [k1 v1] m IH]; intros.
+    - simpl; intros abs; inv abs. 
+    - simpl; flatten_goal.
+      + unfold alist_In; simpl.
+        rewrite Bool.negb_true_iff in Heq; rewrite Heq.
+        intros abs; eapply IH; eassumption.
+      + rewrite Bool.negb_false_iff, rel_dec_correct in Heq; subst.
+        intros abs; eapply IH; eauto. 
+  Qed.
+
+  (* Removing a key does not alter other keys *)
+  Lemma In_In_remove_ineq:
+    forall (m : alist K V) (k : K) (v : V) (k' : K),
+      k <> k' ->
+      alist_In k m v ->
+      alist_In k (alist_remove k' m) v.
+  Proof.
+    induction m as [| [? ?] m IH]; intros ?k ?v ?k' ineq IN; [inversion IN |].
+    simpl.
+    flatten_goal.
+    - unfold alist_In in *; simpl in *.
+      rewrite Bool.negb_true_iff, <- neg_rel_dec_correct in Heq.
+      flatten_goal; auto.
+    - unfold alist_In in *; simpl in *.
+      rewrite Bool.negb_false_iff, rel_dec_correct in Heq; subst.
+      flatten_hyp IN; [rewrite rel_dec_correct in Heq; subst; tauto | eapply IH; eauto].
+  Qed.       
+
+  Lemma In_remove_In_ineq:
+    forall (m : alist K V) (k : K) (v : V) (k' : K),
+      alist_In k (alist_remove k' m) v ->
+      alist_In k m v.
+  Proof.
+    induction m as [| [? ?] m IH]; intros ?k ?v ?k' IN; [inversion IN |].
+    simpl in IN; flatten_hyp IN.
+    - unfold alist_In in *; simpl in *.
+      flatten_all; auto.
+      eapply IH; eauto.
+    -rewrite Bool.negb_false_iff, rel_dec_correct in Heq; subst.
+     unfold alist_In; simpl. 
+     flatten_goal; [rewrite rel_dec_correct in Heq; subst |].
+     exfalso; eapply not_In_remove; eauto.
+     eapply IH; eauto.
+  Qed.       
+
+  Lemma In_remove_In_ineq_iff:
+    forall (m : alist K V) (k : K) (v : V) (k' : K),
+      k <> k' ->
+      alist_In k (alist_remove k' m) v <->
+      alist_In k m v.
+  Proof.
+    intros; split; eauto using In_In_remove_ineq, In_remove_In_ineq.
+  Qed.       
+
+  (* Adding a value to a key does not alter other keys *)
+  Lemma In_In_add_ineq:
+    forall k v k' v' (m: alist K V),
+      k <> k' ->
+      alist_In k m v ->
+      alist_In k (alist_add k' v' m) v.
+  Proof.
+    intros.
+    unfold alist_In; simpl; flatten_goal; [rewrite rel_dec_correct in Heq; subst; tauto |].
+    apply In_In_remove_ineq; auto.
+  Qed.
+
+  Lemma In_add_In_ineq:
+    forall k v k' v' (m: alist K V),
+      k <> k' ->
+      alist_In k (alist_add k' v' m) v ->
+      alist_In k m v. 
+  Proof.
+    intros k v k' v' m ineq IN.
+    unfold alist_In in IN; simpl in IN; flatten_hyp IN; [rewrite rel_dec_correct in Heq; subst; tauto |].
+    eapply In_remove_In_ineq; eauto.
+  Qed.
+
+  Lemma In_add_ineq_iff: 
+    forall m (v v' : V) (k k' : K),
+      k <> k' ->
+      alist_In k m v <-> alist_In k (alist_add k' v' m) v.
+  Proof.
+    intros; split; eauto using In_In_add_ineq, In_add_In_ineq.
+  Qed.
+
+  (* alist_find fails iff no value is associated to the key in the map *)
+  Lemma alist_find_None:
+    forall k (m: alist K V),
+      (forall v, ~ In (k,v) m) <-> alist_find k m = None.
+  Proof.
+    induction m as [| [k1 v1] m IH]; [simpl; easy |].
+    simpl; split; intros H. 
+    - flatten_goal; [rewrite rel_dec_correct in Heq; subst; exfalso | rewrite <- neg_rel_dec_correct in Heq].
+      apply (H v1); left; reflexivity.
+      apply IH; intros v abs; apply (H v); right; assumption.
+    - intros v; flatten_hyp H; [inv H | rewrite <- IH in H].
+      intros [EQ | abs]; [inv EQ; rewrite <- neg_rel_dec_correct in Heq; tauto | apply (H v); assumption]. 
+  Qed.
+
+  Lemma alist_In_add_eq : forall m (k:K) (v n:V), alist_In k (alist_add k n m) v -> n = v.
+  Proof.
+    destruct m as [| [k1 v1]]; intros.
+    - unfold alist_add in H.
+      unfold alist_In in H. simpl in H.
+      destruct (k ?[ eq ] k); inversion H; auto.
+    - unfold alist_add in H.
+      unfold alist_In in H.
+      simpl in H.
+      destruct (k ?[ eq ] k). inversion H; auto.
+      pose proof (@not_In_remove ((k1,v1)::m)).
+      unfold alist_In in H0. simpl in H0.
+      apply H0 in H.
+      contradiction.
+  Qed.
+
+  Lemma alist_find_remove_none:
+    forall (m : list (K*V)) (k1 k2 : K), k2 <> k1 -> alist_find k1 (alist_remove k2 m) = None -> alist_find k1 m = None.
+  Proof.
+    induction m as [| [? ?] m IH]; intros ?k1 ?k2 ineq HF; simpl in *.
+    - reflexivity.
+    - destruct (rel_dec_p k1 k).
+      + subst. eapply rel_dec_neq_false in ineq; eauto. rewrite ineq in HF. simpl in HF.
+        assert (k = k) by reflexivity.
+        apply rel_dec_correct in H. rewrite H in HF. inversion HF.
+      + destruct (rel_dec_p k2 k); simpl in *.
+        apply rel_dec_correct in e. rewrite e in HF. simpl in HF.
+        eapply rel_dec_neq_false in n; eauto. rewrite n. eapply IH. apply ineq. assumption.
+        eapply rel_dec_neq_false in n0; eauto. rewrite n0 in HF. simpl in HF.
+        eapply rel_dec_neq_false in n; eauto. rewrite n in *. eapply IH. apply ineq. assumption.
+  Qed.
+    
+  Lemma alist_find_add_none:
+    forall m (k r :K) (v:V), 
+    alist_find k (alist_add r v m) = None ->
+    alist_find k m = None.
+  Proof.
+    destruct m as [| [k1 v1]]; intros.
+    - reflexivity.
+    - simpl in *.
+      remember (k ?[ eq ] r) as x.
+      destruct x.  inversion H.
+      remember (r ?[ eq] k1) as y.
+      destruct y. simpl in *. symmetry in Heqy. rewrite rel_dec_correct in Heqy. subst.
+      rewrite <- Heqx.
+      apply (alist_find_remove_none _ k k1); auto.
+      rewrite rel_dec_sym in Heqx; eauto.
+      apply neg_rel_dec_correct. symmetry in Heqx. assumption.
+      simpl in H.
+      destruct (k ?[ eq ] k1); auto.
+      apply (alist_find_remove_none _ k r); auto.
+      rewrite rel_dec_sym in Heqx; eauto.
+      apply neg_rel_dec_correct. symmetry in Heqx. assumption.
+  Qed.      
+
+  
+  Lemma alist_find_neq : forall m (k r:K) (v:V), k <> r -> alist_find k (alist_add r v m) = alist_find k m.
+  Proof.
+    intros.
+    remember (alist_find k (alist_add r v m)) as x.
+    destruct x.
+    - symmetry in Heqx. apply In_add_In_ineq in Heqx; auto.
+    - symmetry in Heqx. symmetry. eapply alist_find_add_none. apply Heqx.
+ Qed.
+  
+  
+End alistFacts.
+Arguments alist_find {_ _ _ _}.
+Arguments alist_add {_ _ _ _}.
+Arguments alist_find {_ _ _ _}.
+Arguments alist_remove {_ _ _ _}.
